Refactoring

CertifyingDatalog/ModelChecking.lean
@@ -3,17 +3,17 @@ import CertifyingDatalog.Unification
 import Mathlib.Data.Set.Basic
 import CertifyingDatalog.Basic
 
-structure PartialGroundRule (τ: Signature) [DecidableEq τ.vars] [DecidableEq τ.constants] [DecidableEq τ.relationSymbols] [Inhabited τ.constants] [Hashable τ.constants] [Hashable τ.relationSymbols] [Hashable τ.vars] [ToString τ.constants] [ToString τ.vars] [ToString τ.relationSymbols] where
+structure PartialGroundRule (τ: Signature) where
   head: Atom τ
   groundedBody: List (GroundAtom τ)
   ungroundedBody: List (Atom τ)
 
-abbrev CheckableModel (τ: Signature) [DecidableEq τ.vars] [DecidableEq τ.constants] [DecidableEq τ.relationSymbols] [Inhabited τ.constants] [Hashable τ.constants] [Hashable τ.relationSymbols] [Hashable τ.vars] [ToString τ.constants] [ToString τ.vars] [ToString τ.relationSymbols] := List (GroundAtom τ)
+abbrev CheckableModel (τ: Signature) := List (GroundAtom τ)
 
-variable {τ: Signature} [DecidableEq τ.vars] [DecidableEq τ.constants] [DecidableEq τ.relationSymbols] [Inhabited τ.constants]  [Hashable τ.constants] [Hashable τ.vars] [Hashable τ.relationSymbols] [ToString τ.constants] [ToString τ.vars] [ToString τ.relationSymbols]
+variable {τ: Signature}
 
 namespace PartialGroundRule
-  def isSafe (pgr: PartialGroundRule τ): Prop :=
+  def isSafe [DecidableEq τ.vars] (pgr: PartialGroundRule τ): Prop :=
     pgr.head.vars ⊆ pgr.ungroundedBody.foldl_union Atom.vars ∅
 
   def isGround (pgr: PartialGroundRule τ): Prop :=
@@ -25,131 +25,138 @@ namespace PartialGroundRule
   def toRule (pgr: PartialGroundRule τ) : Rule τ :=
     {head:= pgr.head, body := (pgr.groundedBody.map GroundAtom.toAtom) ++ pgr.ungroundedBody}
 
-  lemma toRule_inv_fromRule (r: Rule τ): (fromRule r).toRule = r := by
+  lemma toRule_inv_fromRule {r: Rule τ}: (fromRule r).toRule = r := by
     unfold fromRule
     unfold toRule
     simp
 
   def isActive (pgr: PartialGroundRule τ) (i: Interpretation τ) : Prop := ∀ (ga: GroundAtom τ), ga ∈ pgr.groundedBody → ga ∈ i
 
-  lemma fromRule_isActive (r: Rule τ) (i: Interpretation τ) : (fromRule r).isActive i := by
+  lemma fromRule_isActive {r: Rule τ} (i: Interpretation τ) : (fromRule r).isActive i := by
     unfold isActive
     unfold fromRule
     simp
 
-  lemma fromRule_safe_iff_rule_safe (r : Rule τ) : (fromRule r).isSafe ↔ r.isSafe := by
+  lemma fromRule_safe_iff_rule_safe [DecidableEq τ.vars] {r : Rule τ} : (fromRule r).isSafe ↔ r.isSafe := by
     unfold isSafe
     unfold Rule.isSafe
     unfold fromRule
     simp
 
-  def isSatisfied (pgr : PartialGroundRule τ) (i : Interpretation τ) : Prop := ∀ (g : Grounding τ), i.satisfiesRule (g.applyRule' pgr.toRule)
+  def isSatisfied [DecidableEq τ.constants] [DecidableEq τ.vars] [DecidableEq τ.relationSymbols] (pgr : PartialGroundRule τ) (i : Interpretation τ) : Prop := ∀ (g : Grounding τ), i.satisfiesRule (g.applyRule' pgr.toRule)
 
-  lemma satisfied_iff_of_eq_toRule (pgr1 pgr2: PartialGroundRule τ) (i: Interpretation τ) (h: pgr1.toRule = pgr2.toRule): pgr1.isSatisfied i ↔ pgr2.isSatisfied i := by
+  lemma satisfied_iff_of_eq_toRule [DecidableEq τ.constants] [DecidableEq τ.vars] [DecidableEq τ.relationSymbols]
+      (pgr1 pgr2: PartialGroundRule τ) (i: Interpretation τ) (h: pgr1.toRule = pgr2.toRule): pgr1.isSatisfied i ↔ pgr2.isSatisfied i := by
     unfold isSatisfied
     simp only [h]
 
-  lemma head_noVars_of_safe_of_ground (pgr : PartialGroundRule τ) : pgr.isSafe -> pgr.isGround -> pgr.head.vars = ∅ := by
+  lemma head_noVars_of_safe_of_ground [DecidableEq τ.vars] (pgr : PartialGroundRule τ) : pgr.isSafe -> pgr.isGround -> pgr.head.vars = ∅ := by
     unfold isSafe
     unfold isGround
     intro safe ground
     rw [ground] at safe
     unfold List.foldl_union at safe
-    simp at safe
+    simp only [List.foldl_nil, Finset.subset_empty] at safe
     apply Finset.Subset.antisymm
-    rw [safe]
-    simp
+    · rw [safe]
+    · simp
 
 end PartialGroundRule
 
 namespace Grounding
   def applyPartialGroundRule (g : Grounding τ) (pgr : PartialGroundRule τ) : GroundRule τ := g.applyRule' pgr.toRule
 
-  lemma applyPartialGroundRule_eq_apply_only_ungrounded (g : Grounding τ) (pgr : PartialGroundRule τ) :
+  lemma applyPartialGroundRule_eq_apply_only_ungrounded {g : Grounding τ} {pgr : PartialGroundRule τ} :
     g.applyPartialGroundRule pgr = { head := g.applyAtom' pgr.head, body := pgr.groundedBody ++ pgr.ungroundedBody.map g.applyAtom'} := by
     unfold applyPartialGroundRule
     unfold applyRule'
-    simp [PartialGroundRule.toRule]
+    simp only [PartialGroundRule.toRule, List.map_append, List.map_map, GroundRule.mk.injEq,
+      List.append_cancel_right_eq, true_and]
     apply List.ext_getElem
     · rw [List.length_map]
     · intro _ _ _
-      simp
+      simp only [List.getElem_map, Function.comp_apply]
       rw [applyAtom'_on_GroundAtom_unchanged]
 end Grounding
 
 namespace PartialGroundRule
-  lemma satisfied_of_not_active (pgr: PartialGroundRule τ) (i: Interpretation τ) : ¬ pgr.isActive i -> pgr.isSatisfied i := by
+  variable [DecidableEq τ.constants] [DecidableEq τ.vars] [DecidableEq τ.relationSymbols]
+
+  lemma satisfied_of_not_active {pgr: PartialGroundRule τ} {i: Interpretation τ} : ¬ pgr.isActive i -> pgr.isSatisfied i := by
     intro notActive
     unfold isSatisfied
     intro g
     unfold Interpretation.satisfiesRule
     intro h
     unfold isActive at notActive
-    simp at notActive
-    have apply_eq := g.applyPartialGroundRule_eq_apply_only_ungrounded pgr
+    simp only [not_forall, Classical.not_imp] at notActive
+    have apply_eq := @ g.applyPartialGroundRule_eq_apply_only_ungrounded τ pgr
     unfold Grounding.applyPartialGroundRule at apply_eq
     rw [apply_eq] at h
     unfold GroundRule.bodySet at h
-    simp at h
+    simp only [List.toFinset_append, Finset.coe_union, List.coe_toFinset, List.mem_map,
+      Set.union_subset_iff] at h
     rcases notActive with ⟨a, a_mem_body, a_not_mem_i⟩
     apply False.elim
     apply a_not_mem_i
     apply h.left
-    simp
+    simp only [Set.mem_setOf_eq]
     exact a_mem_body
 end PartialGroundRule
 
 namespace CheckableModel
+  variable [DecidableEq τ.constants] [DecidableEq τ.vars] [DecidableEq τ.relationSymbols]
+
   def substitutionsForAtom (m : CheckableModel τ) (a : Atom τ) : List (Substitution τ) := m.filterMap (fun ga => Substitution.empty.matchAtom a ga)
 
-  lemma noVars_after_applying_substitutionsForAtom (m : CheckableModel τ) (a : Atom τ) : ∀ s ∈ m.substitutionsForAtom a, (s.applyAtom a).vars = ∅ := by
+  lemma noVars_after_applying_substitutionsForAtom {m : CheckableModel τ} {a : Atom τ} : ∀ s ∈ m.substitutionsForAtom a, (s.applyAtom a).vars = ∅ := by
     unfold substitutionsForAtom
     intro s s_mem
-    simp at s_mem
+    simp only [List.mem_filterMap] at s_mem
     rcases s_mem with ⟨ga, _, ga_eq⟩
     have : s = (Substitution.empty.matchAtom a ga).get (by simp [ga_eq]) := by simp [ga_eq]
     rw [this]
     rw [Substitution.matchAtomYieldsSubs]
     exact ga.vars_empty
 
-  lemma substitutionsForAtom_application_in_model (m : CheckableModel τ) (a : Atom τ) : ∀ (h : s ∈ m.substitutionsForAtom a), (s.applyAtom a).toGroundAtom (m.noVars_after_applying_substitutionsForAtom a s h) ∈ m := by
+  lemma substitutionsForAtom_application_in_model {m : CheckableModel τ} {a : Atom τ} : ∀ (h : s ∈ m.substitutionsForAtom a), (s.applyAtom a).toGroundAtom (m.noVars_after_applying_substitutionsForAtom s h) ∈ m := by
     intro h
     unfold substitutionsForAtom at h
-    simp at h
+    simp only [List.mem_filterMap] at h
     rcases h with ⟨ga, ga_mem, ga_eq⟩
     have : s = (Substitution.empty.matchAtom a ga).get (by simp [ga_eq]) := by simp [ga_eq]
-    simp [this]
-    simp [Substitution.matchAtomYieldsSubs]
+    simp only [this]
+    simp only [Substitution.matchAtomYieldsSubs]
     have : ga = ga.toAtom.toGroundAtom ga.vars_empty := by rw [GroundAtom.eq_iff_toAtom_eq]; rw [← ga.toAtom.toGroundAtom_isSelf]
     rw [← this]
     exact ga_mem
 
-  lemma mem_substitutionsForAtom_iff (m : CheckableModel τ) (a : Atom τ) :
+  lemma mem_substitutionsForAtom_iff {m : CheckableModel τ} {a : Atom τ} :
     ∀ (s : Substitution τ), s ∈ m.substitutionsForAtom a ↔ ∃ ga ∈ m, s.applyAtom a = ga ∧ ∀ (s': Substitution τ), s'.applyAtom a = ga → s ⊆ s' := by
     intro s
     constructor
     · intro h
-      exists (s.applyAtom a).toGroundAtom (m.noVars_after_applying_substitutionsForAtom a s h)
+      exists (s.applyAtom a).toGroundAtom (m.noVars_after_applying_substitutionsForAtom s h)
       constructor
       · apply substitutionsForAtom_application_in_model; exact h
-      rw [← Atom.toGroundAtom_isSelf]
-      simp
-      intro s' eq
+      · rw [← Atom.toGroundAtom_isSelf]
+        simp
+        intro s' eq
 
-      unfold substitutionsForAtom at h
-      simp at h
-      rcases h with ⟨ga, _, ga_eq⟩
-      have : s = (Substitution.empty.matchAtom a ga).get (by simp [ga_eq]) := by simp [ga_eq]
+        unfold substitutionsForAtom at h
+        simp only [List.mem_filterMap] at h
+        rcases h with ⟨ga, _, ga_eq⟩
+        have : s = (Substitution.empty.matchAtom a ga).get (by simp [ga_eq]) := by simp [ga_eq]
 
-      rw [this]
-      apply Substitution.matchAtomIsMinimal
-      constructor
-      · apply Substitution.empty_isMinimal
-      · rw [eq, this]; rw [Substitution.matchAtomYieldsSubs]
+        rw [this]
+        apply Substitution.matchAtomIsMinimal
+        constructor
+        · apply Substitution.empty_isMinimal
+        · rw [eq, this]; rw [Substitution.matchAtomYieldsSubs]
     · intro h
       rcases h with ⟨ga, mem, ga_eq, minimal⟩
       unfold substitutionsForAtom
-      simp
+      simp only [List.mem_filterMap]
       exists ga
       constructor
       · exact mem
@@ -158,7 +165,6 @@ namespace CheckableModel
           simp
           apply @Substitution.matchAtomNoneThenNoSubs τ
           rw [eq]
-          simp
           apply Substitution.empty_isMinimal
           apply ga_eq
         | some s' =>
@@ -173,6 +179,8 @@ namespace CheckableModel
           · apply minimal
             rw [this]
             apply Substitution.matchAtomYieldsSubs
+
+  variable [ToString τ.constants] [ToString τ.vars] [ToString τ.relationSymbols]
 
   def checkPGR (m : CheckableModel τ) (pgr : PartialGroundRule τ) (safe : pgr.isSafe) : Except String Unit :=
     match eq : pgr.ungroundedBody with
@@ -200,13 +208,13 @@ namespace CheckableModel
             exact v_in_adj_head.right
 
           rw [eq] at this
-          simp [List.foldl_union] at this
+          simp only [List.foldl_union, List.foldl_cons, Finset.empty_union] at this
           have mem_foldl_union := @List.mem_foldl_union (Atom τ) τ.vars
-          simp [List.foldl_union] at mem_foldl_union
+          simp only [List.foldl_union] at mem_foldl_union
           rw [mem_foldl_union] at this
           cases this with
           | inl v_in_hd =>
-            have noVars_in_hd := m.noVars_after_applying_substitutionsForAtom hd s s_mem
+            have noVars_in_hd := m.noVars_after_applying_substitutionsForAtom s s_mem
             have v_in_applied_hd : v ∈ (s.applyAtom hd).vars := by
               rw [Substitution.applyAtom_remainingVarsNotInDomain]
               rw [Finset.mem_filter_nc]
@@ -232,276 +240,292 @@ namespace CheckableModel
       )
   termination_by pgr.ungroundedBody.length
 
-  lemma checkPGRIsOkIffRuleIsSatisfied (m : CheckableModel τ) (pgr : PartialGroundRule τ) (safe : pgr.isSafe) (active : pgr.isActive m.toSet) : m.checkPGR pgr safe = Except.ok () ↔ pgr.isSatisfied m.toSet := by
+  lemma checkPGRIsOkIffRuleIsSatisfied [Inhabited τ.constants] {m : CheckableModel τ} {pgr : PartialGroundRule τ} (safe : pgr.isSafe) (active : pgr.isActive m.toSet) : m.checkPGR pgr safe = Except.ok () ↔ pgr.isSatisfied m.toSet := by
     unfold checkPGR
     split
-    case h_1 heq =>
-      have : ∀ g : Grounding τ, g.applyAtom' pgr.head = pgr.head.toGroundAtom (pgr.head_noVars_of_safe_of_ground safe heq) := by
-        intro g
-        rw [GroundAtom.eq_iff_toAtom_eq]
-        rw [g.applyAtom'_on_Atom_without_vars_unchanged (pgr.head_noVars_of_safe_of_ground safe heq)]
-        rw [← Atom.toGroundAtom_isSelf]
-      split
-      case isTrue h =>
-        simp
-        unfold PartialGroundRule.isSatisfied
-        unfold Interpretation.satisfiesRule
-        intro g _
-        unfold Grounding.applyRule'
-        unfold PartialGroundRule.toRule
-        simp
-        rw [this]
-        unfold List.toSet
-        simp
-        exact h
-      case isFalse h =>
-        simp
-        unfold PartialGroundRule.isSatisfied
-        unfold Interpretation.satisfiesRule
-        unfold Grounding.applyRule'
-        unfold PartialGroundRule.toRule
-        rw [heq]
-        simp
-        let g : Grounding τ := (fun _ => Inhabited.default (α := τ.constants))
-        exists g
-        unfold GroundRule.bodySet
-        simp
-        constructor
-        · unfold PartialGroundRule.isActive at active
-          intro a a_mem
-          simp at a_mem
-          apply active
-          rcases a_mem with ⟨a', a'_mem, a'_eq⟩
-          rw [g.applyAtom'_on_GroundAtom_unchanged] at a'_eq
-          rw [a'_eq] at a'_mem
-          exact a'_mem
-        · rw[this]
-          unfold List.toSet
+    · case h_1 heq =>
+        have : ∀ g : Grounding τ, g.applyAtom' pgr.head = pgr.head.toGroundAtom (pgr.head_noVars_of_safe_of_ground safe heq) := by
+          intro g
+          rw [GroundAtom.eq_iff_toAtom_eq]
+          rw [g.applyAtom'_on_Atom_without_vars_unchanged (pgr.head_noVars_of_safe_of_ground safe heq)]
+          rw [← Atom.toGroundAtom_isSelf]
+        split
+        case isTrue h =>
           simp
+          unfold PartialGroundRule.isSatisfied
+          unfold Interpretation.satisfiesRule
+          intro g _
+          unfold Grounding.applyRule'
+          unfold PartialGroundRule.toRule
+          simp only
+          rw [this]
+          unfold List.toSet
+          simp only [List.coe_toFinset, Set.mem_setOf_eq]
           exact h
-    case h_2 hd tl heq =>
-      rw [List.mapExceptUnit_iff]
-      simp
-      unfold PartialGroundRule.isSatisfied
-      unfold Interpretation.satisfiesRule
-
-      constructor
-      · intro subs_works
-        unfold Grounding.applyRule'
-        unfold PartialGroundRule.toRule
-        unfold GroundRule.bodySet
-        simp
-        intro g g_active_grounded g_active_ungrounded
-        unfold List.toSet at g_active_grounded
-        simp at g_active_grounded
-        rw [heq] at g_active_ungrounded
-        unfold List.toSet at g_active_ungrounded
-        simp at g_active_ungrounded
-
-        let subs : Substitution τ := (fun v => if v ∈ hd.vars then g v else Option.none)
-
-        have g_after_subs : ∀ a, g.applyAtom' (subs.applyAtom a) = g.applyAtom' a := by
-          intro a
-          unfold Substitution.applyAtom
-          unfold Grounding.applyAtom'
+        case isFalse h =>
           simp
-          intro t t_mem
-          unfold Substitution.applyTerm
-          unfold Grounding.applyTerm'
-          cases t with
-          | constant c => simp
-          | variableDL v =>
-            simp [subs]
-            cases Decidable.em (v ∈ hd.vars) with
-            | inl h => simp [h]
-            | inr h => simp [h]
-
-        have g_eq_subs_on_hd : subs.applyAtom hd = g.applyAtom' hd := by
-          unfold Substitution.applyAtom
-          unfold Grounding.applyAtom'
-          unfold GroundAtom.toAtom
-          simp
-          intro t t_mem
-          unfold Substitution.applyTerm
-          unfold Grounding.applyTerm'
-          cases t with
-          | constant c => simp
-          | variableDL v =>
-            have : v ∈ hd.vars := by
-              unfold Atom.vars
-              rw [List.mem_foldl_union]
-              apply Or.inr
-              exists Term.variableDL v
-              unfold Term.vars
-              constructor
-              · exact t_mem
-              · simp
-            simp [subs, this]
-
-        have subs_domain : subs.domain = hd.vars := by
-          unfold Substitution.domain
-          apply Set.ext
-          intro v
-          simp [subs]
-
-        specialize subs_works subs (by
-          rw [mem_substitutionsForAtom_iff]
-          exists g.applyAtom' hd
+          unfold PartialGroundRule.isSatisfied
+          unfold Interpretation.satisfiesRule
+          unfold Grounding.applyRule'
+          unfold PartialGroundRule.toRule
+          rw [heq]
+          simp only [List.append_nil, List.map_map, not_forall, Classical.not_imp]
+          let g : Grounding τ := (fun _ => Inhabited.default (α := τ.constants))
+          exists g
+          unfold GroundRule.bodySet
+          simp only [List.coe_toFinset, List.mem_map, Function.comp_apply]
           constructor
-          · apply g_active_ungrounded; apply Or.inl; rfl
-          constructor
-          · exact g_eq_subs_on_hd
-          · intro s' s'_apply_also_ground
-            rw [← g_eq_subs_on_hd] at s'_apply_also_ground
-            intro v v_in_dom
-            rw [subs_domain] at v_in_dom
-            simp at v_in_dom
-            unfold Substitution.applyAtom at s'_apply_also_ground
-            simp at s'_apply_also_ground
-            specialize s'_apply_also_ground (Term.variableDL v) (by
-              unfold Atom.vars at v_in_dom
-              rw [List.mem_foldl_union] at v_in_dom
-              cases v_in_dom; contradiction;
-              case inr h =>
-              rcases h with ⟨t, t_mem, v_in_t⟩
-              unfold Term.vars at v_in_t
-              cases t <;> simp at v_in_t
-              rw [v_in_t]
-              exact t_mem
-            )
-            unfold Substitution.applyTerm at s'_apply_also_ground
-            simp [subs, v_in_dom] at s'_apply_also_ground
-            simp [subs, v_in_dom]
-            cases eq : s' v with
-            | none => simp [eq] at s'_apply_also_ground
-            | some c =>
-              simp [eq] at s'_apply_also_ground
-              rw [s'_apply_also_ground]
-        )
-        have _termination : tl.length < pgr.ungroundedBody.length := by rw [heq]; simp
-        rw [m.checkPGRIsOkIffRuleIsSatisfied _ _ (by
-          unfold PartialGroundRule.isActive
-          unfold List.toSet
-          simp
-          intro ga ga_eq
-          cases ga_eq with
-          | inl ga_eq =>
-            specialize g_active_grounded ga
-            rw [Grounding.applyAtom'_on_GroundAtom_unchanged] at g_active_grounded
-            apply g_active_grounded
-            exact ga_eq
-          | inr ga_eq =>
-            apply g_active_ungrounded
-            apply Or.inl
-            rw [ga_eq]
-            rw [GroundAtom.eq_iff_toAtom_eq]
-            rw [← Atom.toGroundAtom_isSelf]
-            rw [g_eq_subs_on_hd]
-        )] at subs_works
-        unfold PartialGroundRule.isSatisfied at subs_works
-        unfold Interpretation.satisfiesRule at subs_works
-        unfold PartialGroundRule.toRule at subs_works
-        unfold GroundRule.bodySet at subs_works
-        unfold Grounding.applyRule' at subs_works
-        simp at subs_works
-        specialize subs_works g
-        rw [g_after_subs] at subs_works
-        apply subs_works
-        unfold List.toSet
-        rw [Set.subset_def]
-        simp
-        constructor
-        · rw [← (subs.applyAtom hd).toGroundAtom_isSelf]; rw [g_after_subs]; apply g_active_ungrounded; apply Or.inl; rfl
-        intro a h
-        cases h with
-        | inl h =>
-          rcases h with ⟨b, h⟩
-          rw [← h.right]
-          apply g_active_grounded
-          exact h.left
-        | inr h =>
-          rcases h with ⟨b, h⟩
-          rw [← h.right]
-          apply g_active_ungrounded
-          apply Or.inr
-          exists b
-          rw [g_after_subs]
-          simp
-          exact h.left
-      · intro grounding_works
-        intro subs subs_mem
-        have _termination : tl.length < pgr.ungroundedBody.length := by rw [heq]; simp
-        rw [m.checkPGRIsOkIffRuleIsSatisfied _ _ (by
-          unfold PartialGroundRule.isActive
-          unfold List.toSet
-          simp
-          intro ga h
-          cases h with
-          | inl h =>
-            unfold PartialGroundRule.isActive at active
-            unfold List.toSet at active
-            simp at active
-            apply active
+          · rw[this]
+            unfold List.toSet
+            simp only [List.coe_toFinset, Set.mem_setOf_eq]
             exact h
-          | inr h =>
-            rw [h]
-            apply substitutionsForAtom_application_in_model
-            exact subs_mem
-        )]
+          · unfold PartialGroundRule.isActive at active
+            intro a a_mem
+            simp only [Set.mem_setOf_eq] at a_mem
+            apply active
+            rcases a_mem with ⟨a', a'_mem, a'_eq⟩
+            rw [g.applyAtom'_on_GroundAtom_unchanged] at a'_eq
+            rw [a'_eq] at a'_mem
+            exact a'_mem
+    · case h_2 hd tl heq =>
+        rw [List.mapExceptUnit_iff]
+        simp
         unfold PartialGroundRule.isSatisfied
         unfold Interpretation.satisfiesRule
-        unfold Grounding.applyRule'
-        unfold PartialGroundRule.toRule
-        unfold List.toSet
-        unfold GroundRule.bodySet
-        simp
-        intro g h
-        rw [Set.subset_def] at h
-        simp at h
-        unfold List.toSet at grounding_works
-        unfold PartialGroundRule.toRule at grounding_works
-        unfold Grounding.applyRule' at grounding_works
-        unfold GroundRule.bodySet at grounding_works
-        simp at grounding_works
 
-        let grounding : Grounding τ := fun v => (subs v).getD (g v)
-
-        have : ∀ a, grounding.applyAtom' a = g.applyAtom' (subs.applyAtom a) := by
-          intro a
-          simp [grounding]
-          unfold Grounding.applyAtom'
-          unfold Substitution.applyAtom
-          simp
-          intro t t_mem
-          unfold Substitution.applyTerm
-          unfold Grounding.applyTerm'
-          cases t with
-          | constant _ => simp
-          | variableDL v => simp; cases subs v <;> simp
-
-        specialize grounding_works grounding
-        rw [this] at grounding_works
-        apply grounding_works
-        intro ga ga_mem
-        rw [Grounding.applyAtom'_on_GroundAtom_unchanged]
-        apply h.right
-        apply Or.inl
-        exists ga
-        rw [Grounding.applyAtom'_on_GroundAtom_unchanged]
-        simp
-        exact ga_mem
-        rw [heq]
-        rw [← Atom.toGroundAtom_isSelf] at h
-        simp
         constructor
-        · rw [this]; exact h.left
-        intro a a_mem
-        apply h.right
-        apply Or.inr
-        exists a
-        rw [this]
-        simp
-        exact a_mem
+        · intro subs_works
+          unfold Grounding.applyRule'
+          unfold PartialGroundRule.toRule
+          unfold GroundRule.bodySet
+          simp only [List.map_append, List.map_map, List.toFinset_append, Finset.coe_union,
+            List.coe_toFinset, List.mem_map, Function.comp_apply, Set.union_subset_iff, and_imp]
+          intro g g_active_grounded g_active_ungrounded
+          unfold List.toSet at g_active_grounded
+          simp only [List.coe_toFinset, Set.setOf_subset_setOf, forall_exists_index, and_imp,
+            forall_apply_eq_imp_iff₂] at g_active_grounded
+          rw [heq] at g_active_ungrounded
+          unfold List.toSet at g_active_ungrounded
+          simp only [List.mem_cons, exists_eq_or_imp, List.coe_toFinset,
+            Set.setOf_subset_setOf] at g_active_ungrounded
+
+          let subs : Substitution τ := (fun v => if v ∈ hd.vars then g v else Option.none)
+
+          have g_after_subs : ∀ a, g.applyAtom' (subs.applyAtom a) = g.applyAtom' a := by
+            intro a
+            unfold Substitution.applyAtom
+            unfold Grounding.applyAtom'
+            simp only [List.map_map, GroundAtom.mk.injEq, List.map_inj_left, Function.comp_apply,
+              true_and]
+            intro t t_mem
+            unfold Substitution.applyTerm
+            unfold Grounding.applyTerm'
+            cases t with
+            | constant c => simp
+            | variableDL v =>
+              simp only [subs]
+              cases Decidable.em (v ∈ hd.vars) with
+              | inl h => simp [h]
+              | inr h => simp [h]
+
+          have g_eq_subs_on_hd : subs.applyAtom hd = g.applyAtom' hd := by
+            unfold Substitution.applyAtom
+            unfold Grounding.applyAtom'
+            unfold GroundAtom.toAtom
+            simp only [List.map_map, Atom.mk.injEq, List.map_inj_left, Function.comp_apply,
+              true_and, subs]
+            intro t t_mem
+            unfold Substitution.applyTerm
+            unfold Grounding.applyTerm'
+            cases t with
+            | constant c => simp
+            | variableDL v =>
+              have : v ∈ hd.vars := by
+                unfold Atom.vars
+                rw [List.mem_foldl_union]
+                apply Or.inr
+                exists Term.variableDL v
+                unfold Term.vars
+                constructor
+                · exact t_mem
+                · simp only [Finset.mem_singleton, subs]
+              simp [subs, this]
+
+          have subs_domain : subs.domain = hd.vars := by
+            unfold Substitution.domain
+            apply Set.ext
+            intro v
+            simp only [Option.isSome_ite, Finset.setOf_mem, Finset.mem_coe, subs]
+
+          specialize subs_works subs (by
+            rw [mem_substitutionsForAtom_iff]
+            exists g.applyAtom' hd
+            constructor
+            · apply g_active_ungrounded; apply Or.inl; rfl
+            constructor
+            · exact g_eq_subs_on_hd
+            · intro s' s'_apply_also_ground
+              rw [← g_eq_subs_on_hd] at s'_apply_also_ground
+              intro v v_in_dom
+              rw [subs_domain] at v_in_dom
+              simp only [Finset.mem_coe, subs] at v_in_dom
+              unfold Substitution.applyAtom at s'_apply_also_ground
+              simp only [Atom.mk.injEq, List.map_inj_left, true_and, subs] at s'_apply_also_ground
+              specialize s'_apply_also_ground (Term.variableDL v) (by
+                unfold Atom.vars at v_in_dom
+                rw [List.mem_foldl_union] at v_in_dom
+                cases v_in_dom; contradiction;
+                case inr h =>
+                rcases h with ⟨t, t_mem, v_in_t⟩
+                unfold Term.vars at v_in_t
+                cases t <;> simp at v_in_t
+                rw [v_in_t]
+                exact t_mem
+              )
+              unfold Substitution.applyTerm at s'_apply_also_ground
+              simp only [v_in_dom, ↓reduceIte, subs] at s'_apply_also_ground
+              simp only [v_in_dom, ↓reduceIte, subs]
+              cases eq : s' v with
+              | none => simp [eq] at s'_apply_also_ground
+              | some c =>
+                simp only [eq, Term.constant.injEq, subs] at s'_apply_also_ground
+                rw [s'_apply_also_ground]
+          )
+          have _termination : tl.length < pgr.ungroundedBody.length := by rw [heq]; simp
+          rw [m.checkPGRIsOkIffRuleIsSatisfied _ (by
+            unfold PartialGroundRule.isActive
+            unfold List.toSet
+            simp
+            intro ga ga_eq
+            cases ga_eq with
+            | inl ga_eq =>
+              specialize g_active_grounded ga
+              rw [Grounding.applyAtom'_on_GroundAtom_unchanged] at g_active_grounded
+              apply g_active_grounded
+              exact ga_eq
+            | inr ga_eq =>
+              apply g_active_ungrounded
+              apply Or.inl
+              rw [ga_eq]
+              rw [GroundAtom.eq_iff_toAtom_eq]
+              rw [← Atom.toGroundAtom_isSelf]
+              rw [g_eq_subs_on_hd]
+          )] at subs_works
+          unfold PartialGroundRule.isSatisfied at subs_works
+          unfold Interpretation.satisfiesRule at subs_works
+          unfold PartialGroundRule.toRule at subs_works
+          unfold GroundRule.bodySet at subs_works
+          unfold Grounding.applyRule' at subs_works
+          simp only [List.map_append, List.map_cons, List.map_nil, List.append_assoc,
+            List.singleton_append, List.map_map, List.toFinset_append, List.toFinset_cons,
+            Finset.union_insert, Finset.coe_insert, Finset.coe_union, List.coe_toFinset,
+            List.mem_map, Function.comp_apply, subs] at subs_works
+          specialize subs_works g
+          rw [g_after_subs] at subs_works
+          apply subs_works
+          unfold List.toSet
+          rw [Set.subset_def]
+          simp only [Set.mem_insert_iff, Set.mem_union, Set.mem_setOf_eq, List.coe_toFinset,
+            forall_eq_or_imp, subs]
+          constructor
+          · rw [← (subs.applyAtom hd).toGroundAtom_isSelf]; rw [g_after_subs]; apply g_active_ungrounded; apply Or.inl; rfl
+          · intro a h
+            cases h with
+            | inl h =>
+              rcases h with ⟨b, h⟩
+              rw [← h.right]
+              apply g_active_grounded
+              exact h.left
+            | inr h =>
+              rcases h with ⟨b, h⟩
+              rw [← h.right]
+              apply g_active_ungrounded
+              apply Or.inr
+              exists b
+              rw [g_after_subs]
+              simp only [and_true, subs]
+              exact h.left
+        · intro grounding_works
+          intro subs subs_mem
+          have _termination : tl.length < pgr.ungroundedBody.length := by rw [heq]; simp
+          rw [m.checkPGRIsOkIffRuleIsSatisfied _ (by
+            unfold PartialGroundRule.isActive
+            unfold List.toSet
+            simp only [List.mem_append, List.mem_singleton, List.coe_toFinset, Set.mem_setOf_eq]
+            intro ga h
+            cases h with
+            | inl h =>
+              unfold PartialGroundRule.isActive at active
+              unfold List.toSet at active
+              simp only [List.coe_toFinset, Set.mem_setOf_eq] at active
+              apply active
+              exact h
+            | inr h =>
+              rw [h]
+              apply substitutionsForAtom_application_in_model
+              exact subs_mem
+          )]
+          unfold PartialGroundRule.isSatisfied
+          unfold Interpretation.satisfiesRule
+          unfold Grounding.applyRule'
+          unfold PartialGroundRule.toRule
+          unfold List.toSet
+          unfold GroundRule.bodySet
+          simp only [List.map_append, List.map_cons, List.map_nil, List.append_assoc,
+            List.singleton_append, List.map_map, List.toFinset_append, List.toFinset_cons,
+            Finset.union_insert, Finset.coe_insert, Finset.coe_union, List.coe_toFinset,
+            List.mem_map, Function.comp_apply, Set.mem_setOf_eq]
+          intro g h
+          rw [Set.subset_def] at h
+          simp only [Set.mem_insert_iff, Set.mem_union, Set.mem_setOf_eq, forall_eq_or_imp] at h
+          unfold List.toSet at grounding_works
+          unfold PartialGroundRule.toRule at grounding_works
+          unfold Grounding.applyRule' at grounding_works
+          unfold GroundRule.bodySet at grounding_works
+          simp only [List.map_append, List.map_map, List.toFinset_append, Finset.coe_union,
+            List.coe_toFinset, List.mem_map, Function.comp_apply, Set.union_subset_iff,
+            Set.setOf_subset_setOf, forall_exists_index, and_imp, forall_apply_eq_imp_iff₂,
+            Set.mem_setOf_eq] at grounding_works
+
+          let grounding : Grounding τ := fun v => (subs v).getD (g v)
+
+          have : ∀ a, grounding.applyAtom' a = g.applyAtom' (subs.applyAtom a) := by
+            intro a
+            simp only [grounding]
+            unfold Grounding.applyAtom'
+            unfold Substitution.applyAtom
+            simp only [List.map_map, GroundAtom.mk.injEq, List.map_inj_left, Function.comp_apply,
+              true_and, grounding]
+            intro t t_mem
+            unfold Substitution.applyTerm
+            unfold Grounding.applyTerm'
+            cases t with
+            | constant _ => simp
+            | variableDL v => simp; cases subs v <;> simp
+
+          specialize grounding_works grounding
+          rw [this] at grounding_works
+          apply grounding_works
+          · intro ga ga_mem
+            rw [Grounding.applyAtom'_on_GroundAtom_unchanged]
+            apply h.right
+            apply Or.inl
+            exists ga
+            rw [Grounding.applyAtom'_on_GroundAtom_unchanged]
+            simp only [and_true, grounding]
+            exact ga_mem
+          · rw [heq]
+            rw [← Atom.toGroundAtom_isSelf] at h
+            simp only [List.mem_cons, forall_eq_or_imp]
+            constructor
+            · rw [this]; exact h.left
+            · intro a a_mem
+              apply h.right
+              apply Or.inr
+              exists a
+              rw [this]
+              simp only [and_true]
+              exact a_mem
   termination_by pgr.ungroundedBody.length
 
   def checkProgram (m : CheckableModel τ) (p : Program τ) (safe : p.isSafe) : Except String Unit :=
@@ -512,22 +536,23 @@ namespace CheckableModel
       exact r_mem
     ))
 
-  theorem checkProgramIsOkIffAllRulesAreSatisfied (m : CheckableModel τ) (p : Program τ) (safe : p.isSafe) :
+  theorem checkProgramIsOkIffAllRulesAreSatisfied [Inhabited τ.constants] {m : CheckableModel τ} {p : Program τ} (safe : p.isSafe) :
     m.checkProgram p safe = Except.ok () ↔ ∀ r ∈ p.groundProgram, Interpretation.satisfiesRule m.toSet r := by
       unfold checkProgram
       rw [List.mapExceptUnit_iff]
       unfold Program.groundProgram
-      simp
+      simp only [List.mem_attach, forall_const, Subtype.forall, exists_and_left, Set.mem_setOf_eq,
+        forall_exists_index, and_imp]
       constructor
       · intro h gr r r_mem g eq
         specialize h r r_mem
-        rw [m.checkPGRIsOkIffRuleIsSatisfied _ _ (by apply PartialGroundRule.fromRule_isActive)] at h
+        rw [m.checkPGRIsOkIffRuleIsSatisfied _ (by apply PartialGroundRule.fromRule_isActive)] at h
         unfold PartialGroundRule.isSatisfied at h
         rw [PartialGroundRule.toRule_inv_fromRule] at h
         rw [eq]
         apply h
       · intro h r r_mem
-        rw [m.checkPGRIsOkIffRuleIsSatisfied _ _ (by apply PartialGroundRule.fromRule_isActive)]
+        rw [m.checkPGRIsOkIffRuleIsSatisfied _ (by apply PartialGroundRule.fromRule_isActive)]
         unfold PartialGroundRule.isSatisfied
         rw [PartialGroundRule.toRule_inv_fromRule]
         intro g
