CertifyingDatalog/OrderedGraphValidation.lean
@@ -2,15 +2,14 @@ import CertifyingDatalog.Basic
 import CertifyingDatalog.Datalog
 import CertifyingDatalog.TreeValidation
 
-abbrev OrderedProofGraph (τ: Signature) [DecidableEq τ.vars] [DecidableEq τ.constants] [DecidableEq τ.relationSymbols] [Inhabited τ.constants] [Hashable τ.constants] [Hashable τ.vars] [Hashable τ.relationSymbols] [ToString τ.constants] [ToString τ.vars] [ToString τ.relationSymbols] :=
+abbrev OrderedProofGraph (τ: Signature) :=
   { arr : Array ((GroundAtom τ) × List ℕ) // ∀ i : Fin arr.size, ∀ j ∈ arr[i].snd, j < i }
 
-variable {τ: Signature} [DecidableEq τ.vars] [DecidableEq τ.constants] [DecidableEq τ.relationSymbols] [Inhabited τ.constants] [Hashable τ.constants] [Hashable τ.vars] [Hashable τ.relationSymbols] [ToString τ.constants] [ToString τ.vars] [ToString τ.relationSymbols]
-
+variable {τ: Signature}
 namespace OrderedProofGraph
   def labels (G: OrderedProofGraph τ): List (GroundAtom τ) := (Array.map Prod.fst G.val).toList
 
-  lemma in_labels_iff_exists_index (G : OrderedProofGraph τ) (a : GroundAtom τ) : a ∈ G.labels ↔ ∃ i : Fin G.val.size, G.val[i].fst = a := by
+  lemma in_labels_iff_exists_index {G : OrderedProofGraph τ} {a : GroundAtom τ} : a ∈ G.labels ↔ ∃ i : Fin G.val.size, G.val[i].fst = a := by
     unfold labels
     rw [← Array.mem_def, Array.mem_iff_get]
     simp
@@ -32,6 +31,10 @@ namespace OrderedProofGraph
   def isValid (G : OrderedProofGraph τ) (kb : KnowledgeBase τ) : Prop :=
     ∀ i : Fin G.val.size, G.locallyValid kb i
 
+  section checkValidity
+
+  variable [DecidableEq τ.constants] [DecidableEq τ.vars] [DecidableEq τ.relationSymbols] [Hashable τ.vars] [Hashable τ.constants] [Hashable τ.relationSymbols] [ToString τ.constants] [ToString τ.vars] [ToString τ.relationSymbols] [Inhabited τ.constants]
+
   def checkAtIndex (G : OrderedProofGraph τ) (m : SymbolSequenceMap τ) (d : Database τ) (index : Fin G.val.size) : Except String Unit :=
     let predecessors := G.val[index].snd
 
@@ -42,15 +45,15 @@ namespace OrderedProofGraph
         body := G.val[index].snd.attach.map (fun n => (G.val.get n.val (by apply lt_trans; apply G.prop index n.val n.prop; exact index.isLt)).fst)
       }
 
-  lemma checkAtIndexOkIffLocallyValid (G : OrderedProofGraph τ) (kb : KnowledgeBase τ) (i : Fin G.val.size) :
+  lemma checkAtIndexOkIffLocallyValid {G : OrderedProofGraph τ} {kb : KnowledgeBase τ} {i : Fin G.val.size} :
     G.checkAtIndex kb.prog.toSymbolSequenceMap kb.db i = Except.ok () ↔ G.locallyValid kb i := by
       unfold checkAtIndex
-      simp
+      simp only [Array.length_toList, Fin.getElem_fin, List.isEmpty_eq_true, Array.get_eq_getElem]
       split
       case isTrue h =>
         split
         case isTrue h' =>
-          simp
+          simp only [true_iff]
           unfold locallyValid
           apply Or.inl
           constructor; exact h; exact h'
@@ -60,13 +63,14 @@ namespace OrderedProofGraph
           simp [h]
           rw [← List.attach_eq_nil_iff] at h
           rw [h]
-          simp
+          simp only [List.map_nil, iff_or_self]
           intro contra
           contradiction
       case isFalse h =>
         rw [checkRuleMatchOkIffExistsRule]
         unfold locallyValid
-        simp
+        simp only [exists_and_left, Array.length_toList, Fin.getElem_fin, Array.get_eq_getElem,
+          iff_or_self, and_imp]
         intro contra
         contradiction
 
@@ -77,25 +81,26 @@ namespace OrderedProofGraph
       | .ok () => G.checkValidityStep m d (n+1)
     else Except.ok ()
 
-  lemma checkValidityStep_semantics (G : OrderedProofGraph τ) (kb : KnowledgeBase τ) (n : Nat) :
+  lemma checkValidityStep_semantics {G : OrderedProofGraph τ} {kb : KnowledgeBase τ} {n : Nat} :
     G.checkValidityStep kb.prog.toSymbolSequenceMap kb.db n = Except.ok () ↔ ∀ i : Fin G.val.size, n ≤ i.val -> G.locallyValid kb i := by
     unfold checkValidityStep
     split
     case isFalse h =>
-      simp
+      simp only [Array.length_toList, Fin.getElem_fin, true_iff]
       intro i n_leq_i
       have : n < G.val.size := by apply Nat.lt_of_le_of_lt; exact n_leq_i; exact i.isLt
       contradiction
     case isTrue h =>
       split
       case h_1 heq =>
-        simp
+        simp only [reduceCtorEq, Array.length_toList, Fin.getElem_fin, false_iff, not_forall,
+          Classical.not_imp]
         exists ⟨n, h⟩
         constructor
+        · rw [← checkAtIndexOkIffLocallyValid]
+          rw [heq]
+          simp
         · simp
-        rw [← checkAtIndexOkIffLocallyValid]
-        rw [heq]
-        simp
       case h_2 heq =>
         constructor
         · intro next_ok i n_leq_i
@@ -106,7 +111,7 @@ namespace OrderedProofGraph
             rw [this] at heq
             rw [heq]
           | succ j =>
-            apply (G.checkValidityStep_semantics kb (n+1)).mp
+            apply (@G.checkValidityStep_semantics kb (n+1)).mp
             exact next_ok
             rw [Nat.sub_eq_iff_eq_add n_leq_i] at eq
             rw [eq]
@@ -128,16 +133,18 @@ namespace OrderedProofGraph
     unfold isValid
     simp
 
-  def toProofTreeSkeleton (G : OrderedProofGraph τ) (kb : KnowledgeBase τ) (valid : G.isValid kb) (root : Fin G.val.size) : ProofTreeSkeleton τ :=
+  end checkValidity
+
+  def toProofTreeSkeleton {G : OrderedProofGraph τ} {kb : KnowledgeBase τ} (valid : G.isValid kb) (root : Fin G.val.size) : ProofTreeSkeleton τ :=
     let current := G.val[root]
     let next_trees := current.snd.attach.map (fun i =>
       let j : Fin G.val.size := ⟨i.val, by apply lt_trans; apply G.prop root i.val i.prop; exact root.isLt⟩
       have _termination : j.val < root.val := by apply G.prop root j i.prop
-      G.toProofTreeSkeleton kb valid j)
+      G.toProofTreeSkeleton valid j)
     Tree.node current.fst next_trees
   termination_by root
 
-  lemma toProofTreeSkeleton_isValid (G : OrderedProofGraph τ) (kb : KnowledgeBase τ) (valid : G.isValid kb) (root : Fin G.val.size) : (G.toProofTreeSkeleton kb valid root).isValid kb := by
+  lemma toProofTreeSkeleton_isValid (G : OrderedProofGraph τ) (kb : KnowledgeBase τ) (valid : G.isValid kb) (root : Fin G.val.size) : (G.toProofTreeSkeleton valid root).isValid kb := by
     unfold toProofTreeSkeleton
     unfold ProofTreeSkeleton.isValid
     unfold isValid at valid
@@ -145,7 +152,7 @@ namespace OrderedProofGraph
     cases valid root with
     | inl h =>
       apply Or.inr
-      simp
+      simp only [Array.length_toList, Fin.getElem_fin, List.map_eq_nil_iff, List.attach_eq_nil_iff]
       exact h
     | inr h =>
       apply Or.inl
@@ -158,11 +165,12 @@ namespace OrderedProofGraph
       · rw [r_apply]
         simp
         intro a _
-        simp [Tree.root]
+        simp only [Tree.root]
         unfold toProofTreeSkeleton
-        simp
+        simp only [Array.length_toList, Fin.getElem_fin]
       · rw [List.forall_iff_forall_mem]
-        simp
+        simp only [Array.length_toList, Fin.getElem_fin, List.mem_attach, forall_const,
+          Subtype.forall, List.mem_map, true_and, Subtype.exists, forall_exists_index]
         intro t j j_mem next_tree
         rw [← next_tree]
         have _termination : j < root.val := by apply G.prop root j j_mem
@@ -170,12 +178,12 @@ namespace OrderedProofGraph
   termination_by root
 
   def toProofTree (G : OrderedProofGraph τ) (kb : KnowledgeBase τ) (valid : G.isValid kb) (root : Fin G.val.size) : ProofTree kb :=
-    ⟨G.toProofTreeSkeleton kb valid root, G.toProofTreeSkeleton_isValid kb valid root⟩
+    ⟨G.toProofTreeSkeleton valid root, G.toProofTreeSkeleton_isValid kb valid root⟩
 
-  theorem verticesValidOrderedProofGraphAreInProofTheoreticSemantics (G : OrderedProofGraph τ) (kb : KnowledgeBase τ) (valid : G.isValid kb) : G.labels.toSet ⊆ kb.proofTheoreticSemantics := by
+  theorem verticesValidOrderedProofGraphAreInProofTheoreticSemantics [DecidableEq τ.constants] [DecidableEq τ.vars] [DecidableEq τ.relationSymbols] (G : OrderedProofGraph τ) (kb : KnowledgeBase τ) (valid : G.isValid kb) : G.labels.toSet ⊆ kb.proofTheoreticSemantics := by
     unfold KnowledgeBase.proofTheoreticSemantics
     unfold List.toSet
-    simp
+    simp only [List.coe_toFinset, Set.setOf_subset_setOf]
     intro a a_mem
     rw [in_labels_iff_exists_index] at a_mem
     rcases a_mem with ⟨i, h⟩
@@ -184,6 +192,6 @@ namespace OrderedProofGraph
     unfold toProofTreeSkeleton
     unfold ProofTree.root
     unfold Tree.root
-    simp
+    simp only [Array.length_toList, Fin.getElem_fin]
     exact h
 end OrderedProofGraph
